Tests/Chapter_17_Interface.lean
@@ -36,4 +36,10 @@ import CLRSLean.Chapter_17.Section_17_4_Dynamic_Tables
 #check CLRS.Chapter17.dynamicTableInsert_valid
 #check CLRS.Chapter17.dynamicTableInsert_num
 #check CLRS.Chapter17.dynamicTableInsert_amortizedBound
+#check CLRS.Chapter17.dynamicTableDeleteSize
+#check CLRS.Chapter17.dynamicTableDelete
+#check CLRS.Chapter17.dynamicTableDeleteCost
+#check CLRS.Chapter17.dynamicTableDelete_valid
+#check CLRS.Chapter17.dynamicTableDelete_num
+#check CLRS.Chapter17.dynamicTableDelete_amortizedBound
 #check CLRS.Chapter17.dynamicTable_amortizedBound
